theories/LogicalRelation/NormalRed.v
@@ -15,18 +15,24 @@ Program Definition normRedΠ0 {Γ F G l} (h : [Γ ||-Π<l> tProd F G])
   {| PiRedTyPack.dom := F ;
      PiRedTyPack.cod := G |}.
 Solve All Obligations with 
-  intros;
-  assert (wΠ : whnf (tProd F G)) by constructor;
-  pose proof (e := redtywf_whnf (PiRedTyPack.red h) wΠ);
+  intros; pose proof (e := redtywf_whnf (PiRedTyPack.red h) whnf_tProd);
   symmetry in e; injection e; clear e; 
-  destruct h as [?????? domRed codRed codExt] ; 
-  intros; cbn in *; subst; eassumption + now eapply domRed + 
-  (unshelve eapply codRed ; tea ; irrelevance)
-  + ( irrelevance0; [reflexivity| unshelve eapply codExt; tea]; irrelevance).
+  destruct h ; intros; cbn in *; subst; eassumption.
 
-Definition normRedΠ {Γ F G l} (h : [Γ ||-<l> tProd F G])
-  : [Γ ||-<l> tProd F G] :=
+Program Definition normRedΣ0 {Γ F G l} (h : [Γ ||-Σ<l> tSig F G])
+  : [Γ ||-Σ<l> tSig F G] :=
+  {| PiRedTyPack.dom := F ;
+     PiRedTyPack.cod := G |}.
+Solve All Obligations with 
+  intros; pose proof (e := redtywf_whnf (PiRedTyPack.red h) whnf_tSig);
+  symmetry in e; injection e; clear e; 
+  destruct h ; intros; cbn in *; subst; eassumption.
+
+Definition normRedΠ {Γ F G l} (h : [Γ ||-<l> tProd F G]) : [Γ ||-<l> tProd F G] :=
   LRPi' (normRedΠ0 (invLRΠ h)).
+
+Definition normRedΣ {Γ F G l} (h : [Γ ||-<l> tSig F G]) : [Γ ||-<l> tSig F G] :=
+  LRSig' (normRedΣ0 (invLRΣ h)).
 
 #[program]
 Definition normLambda {Γ F F' G t l RΠ} 
@@ -39,26 +45,51 @@ Solve All Obligations with
   destruct Rlam as [????? app eqq]; cbn in *; subst;
   first [eapply app | now eapply eqq| eassumption].
 
+#[program]
+Definition normPair {Γ F F' G G' f g l RΣ} 
+  (Rp : [Γ ||-<l> tPair F' G' f g : tSig F G | normRedΣ RΣ ]) :
+  [Γ ||-<l> tPair F' G' f g : tSig F G | normRedΣ RΣ ] :=
+  {| SigRedTm.nf := tPair F' G' f g |}.
+Solve All Obligations with
+  intros;
+  pose proof (e := redtmwf_whnf (SigRedTm.red Rp) whnf_tPair);
+  destruct Rp as [????? fstRed sndRed]; cbn in *; subst;
+  first [eapply fstRed | irrelevanceRefl; now unshelve eapply sndRed| eassumption].
+
+
 End Normalization.
 
 (** ** Tactics for normalizing the proof relevant components of a reducible type *)
 
 (* Normalizes a term reducible at a Π type *)
 
-Ltac normRedΠin id X :=
+Ltac normRedΠin X :=
   let g := type of X in
   match g with
   | [ LRAd.pack ?R | _ ||- ?t : _] =>
-    pose (id := normRedΠ0 (invLRΠ R));
     let X' := fresh X in
     rename X into X' ;
-    assert (X : [_ ||-<_> t : _ | LRPi' id]) by irrelevance; clear X'
+    assert (X : [_ ||-<_> t : _ | LRPi' (normRedΠ0 (invLRΠ R))]) by irrelevance; clear X'
+  | [ LRAd.pack ?R | _ ||- _ ≅ ?B] =>
+    let X' := fresh X in
+    rename X into X' ;
+    assert (X : [_ ||-<_> _ ≅ B | LRPi' (normRedΠ0 (invLRΠ R))]) by irrelevance; clear X'
+  | [ LRAd.pack ?R | _ ||- ?t ≅ ?u : _] =>
+    let X' := fresh X in
+    rename X into X' ;
+    assert (X : [_ ||-<_> t ≅ u : _ | LRPi' (normRedΠ0 (invLRΠ R))]) by irrelevance; clear X'
   end.
 
-Goal forall `{GenericTypingProperties} Γ A B l R f (Rf : [Γ ||-<l> f : arr A B | R]), True.
+Goal forall `{GenericTypingProperties} Γ A B l R f X
+  (RABX : [Γ ||-<l> arr A B ≅ X | R])
+  (Rf : [Γ ||-<l> f : arr A B | R])
+  (Rff : [Γ ||-<l> f ≅ f : arr A B | R])
+, True.
 Proof.
   intros.
-  normRedΠin ΠAB Rf.
+  normRedΠin Rf.
+  normRedΠin Rff.
+  normRedΠin RABX.
   constructor.
 Qed.
 
@@ -74,3 +105,21 @@ Ltac normRedΠ id :=
     enough [_ ||-<_> t : _ | LRPi' id] by irrelevance
   end.
 
+(* Normalizes a term reducible at a Π type *)
+
+Ltac normRedΣin X :=
+  let g := type of X in
+  match g with
+  | [ LRAd.pack ?R | _ ||- ?t : _] =>
+    let X' := fresh X in
+    rename X into X' ;
+    assert (X : [_ ||-<_> t : _ | LRSig' (normRedΣ0 (invLRΣ R))]) by irrelevance; clear X'
+  | [ LRAd.pack ?R | _ ||- _ ≅ ?B] =>
+    let X' := fresh X in
+    rename X into X' ;
+    assert (X : [_ ||-<_> _ ≅ B | LRSig' (normRedΣ0 (invLRΣ R))]) by irrelevance; clear X'
+  | [ LRAd.pack ?R | _ ||- ?t ≅ ?u : _] =>
+    let X' := fresh X in
+    rename X into X' ;
+    assert (X : [_ ||-<_> t ≅ u : _ | LRSig' (normRedΣ0 (invLRΣ R))]) by irrelevance; clear X'
+  end.
